cleanup notation

Imp/Denot.lean
@@ -50,17 +50,17 @@ def Com.Γ (b: Bexp) (f: State →ˢ State): (State →ˢ State) →o (State →
 
 -- @[simp]
 def Com.denot: Com → (State →ˢ State)
-  | skip      => SRel.id
-  | x ≔ a     => {s | s.2 = s.1⟦x↦a↓s.1⟧}
-  | c;;d      => c.denot ○ d.denot
-  | ife b c d => (c.denot.restrict {s | b↓s = true})
-                  ∪ (d.denot.restrict {s | b↓s = false})
-  | wle b c   => OrderHom.lfp (Γ b c.denot)
+  | skip       => SRel.id
+  | ass x a    => {s | s.2 = s.1⟦x↦a↓s.1⟧}
+  | c;;d       => c.denot ○ d.denot
+  | cond b c d => (c.denot.restrict {s | b↓s = true})
+                    ∪ (d.denot.restrict {s | b↓s = false})
+  | wle b c    => OrderHom.lfp (Γ b c.denot)
 
 notation (priority := high) "⟦" c "⟧" => Com.denot c
 
-#simp (⟦⟧, ⟦"x"↦5⟧⟦"x"↦1⟧) ∈ ⟦⦃x ≔ 5; if x=1 {skip} else {x ≔ 1}⦄⟧
-#simp (⟦⟧, ⟦"x"↦5⟧) ∈ ⟦⦃x ≔ 5; while x=1 {x ≔ 1}⦄⟧
+#simp (⟦⟧, ⟦"x"↦5⟧⟦"x"↦1⟧) ∈ ⟦⦃x = 5; if x == 1 {skip} else {x = 1}⦄⟧
+#simp (⟦⟧, ⟦"x"↦5⟧) ∈ ⟦⦃x = 5; while x == 1 {x = 1}⦄⟧
 
 @[simp]
 instance Com.denot.equiv: Setoid Com where
@@ -77,8 +77,8 @@ theorem Com.denot.cat_congr (hc: c₁ ≈ c₂) (hd: d₁ ≈ d₂):
     simp [HasEquiv.Equiv, denot]
     exact hc ▸ hd ▸ rfl
 
-theorem Com.denot.ife_congr (hc: c₁ ≈ c₂) (hd: d₁ ≈ d₂):
-  (ife b c₁ d₁) ≈ (ife b c₂ d₂) :=
+theorem Com.denot.cond_congr (hc: c₁ ≈ c₂) (hd: d₁ ≈ d₂):
+  (cond b c₁ d₁) ≈ (cond b c₂ d₂) :=
   by
     simp [HasEquiv.Equiv, denot]
     exact hc ▸ hd ▸ rfl
@@ -98,6 +98,6 @@ theorem Com.denot.cat_skipr:
   by simp [HasEquiv.Equiv, denot, SRel.comp]
 
 theorem Com.denot.wle_unfold:
-  wle b c ≈ ife b (c;;wle b c) skip := by
+  wle b c ≈ cond b (c;;wle b c) skip := by
   simp [HasEquiv.Equiv]
   exact Eq.symm (OrderHom.map_lfp (Γ b ⟦c⟧))
