Imp/Syntax.lean
@@ -5,15 +5,6 @@ inductive Aexp
   | sub : Aexp → Aexp → Aexp
   | mul : Aexp → Aexp → Aexp
 
-instance Aexp.Add: Add Aexp where
-  add := add
-
-instance Aexp.Sub: Sub Aexp where
-  sub := sub
-
-instance Aexp.Mul: Mul Aexp where
-  mul := mul
-
 inductive Bexp
   | tt  : Bexp
   | ff  : Bexp
@@ -27,18 +18,11 @@ inductive Com
   | skip  : Com
   | cat   : Com → Com → Com
   | ass   : String → Aexp → Com
-  | ife   : Bexp → Com → Com → Com
+  | cond  : Bexp → Com → Com → Com
   | wle   : Bexp → Com → Com
 
 -- Meta syntax
-notation:60 "¬ₛ" a => Bexp.not a
-notation:70 a₁:70 " =ₛ " a₂:71 => Bexp.eq a₁ a₂
-notation:70 a₁:70 " ≤ₛ " a₂:71 => Bexp.le a₁ a₂
-notation:65 b₁:65 " ∨ₛ " b₂:66 => Bexp.or b₁ b₂
-notation:65 b₁:65 " ∧ₛ " b₂:66 => Bexp.and b₁ b₂
-
 notation:50 x:50 ";;" e:51 => Com.cat x e
-notation:50 x:50 "≔" e:51 => Com.ass x e
 
 -- Syntax of the language
 declare_syntax_cat imp
@@ -52,13 +36,13 @@ syntax:60 imp:60 "+" imp:61 : imp
 syntax:60 imp:60 "-" imp:61 : imp
 syntax:70 imp:70 "*" imp:71 : imp
 -- bexp
-syntax:80 "¬" imp:81 : imp
-syntax:70 imp:70 "=" imp:71 : imp
-syntax:70 imp:70 "≤" imp:71 : imp
-syntax:65 imp:65 "∨" imp:66 : imp
-syntax:65 imp:65 "∧" imp:66 : imp
+syntax:80 "!" imp:81 : imp
+syntax:70 imp:70 "==" imp:71 : imp
+syntax:70 imp:70 "<=" imp:71 : imp
+syntax:65 imp:65 "||" imp:66 : imp
+syntax:65 imp:65 "&&" imp:66 : imp
 -- stmt
-syntax:50 imp:50 "≔" imp:51 : imp
+syntax:50 imp:50 "=" imp:51 : imp
 syntax:40 imp:40 ";" imp:41 : imp
 syntax "if" imp "{" imp "}" "else" "{" imp "}" : imp
 syntax "while" imp "{" imp "}" : imp
@@ -80,21 +64,21 @@ macro_rules
   | `(⦃$x - $y⦄)  => `(Aexp.sub ⦃$x⦄ ⦃$y⦄)
   | `(⦃$x * $y⦄)  => `(Aexp.mul ⦃$x⦄ ⦃$y⦄)
   -- bexp
-  | `(⦃¬$x⦄)      => `(Bexp.not ⦃$x⦄)
-  | `(⦃$x = $y⦄)  => `(Bexp.eq ⦃$x⦄ ⦃$y⦄)
-  | `(⦃$x ≤ $y⦄)  => `(Bexp.le ⦃$x⦄ ⦃$y⦄)
-  | `(⦃$x ∧ $y⦄)  => `(Bexp.and ⦃$x⦄ ⦃$y⦄)
-  | `(⦃$x ∨ $y⦄)  => `(Bexp.or ⦃$x⦄ ⦃$y⦄)
+  | `(⦃!$x⦄)      => `(Bexp.not ⦃$x⦄)
+  | `(⦃$x == $y⦄)  => `(Bexp.eq ⦃$x⦄ ⦃$y⦄)
+  | `(⦃$x <= $y⦄)  => `(Bexp.le ⦃$x⦄ ⦃$y⦄)
+  | `(⦃$x && $y⦄)  => `(Bexp.and ⦃$x⦄ ⦃$y⦄)
+  | `(⦃$x || $y⦄)  => `(Bexp.or ⦃$x⦄ ⦃$y⦄)
   -- stmt
-  | `(⦃$x:ident ≔ $y⦄) => `(Com.ass $(Lean.quote (toString x.getId)) ⦃$y⦄)
+  | `(⦃$x:ident = $y⦄) => `(Com.ass $(Lean.quote (toString x.getId)) ⦃$y⦄)
   | `(⦃$x ; $y⦄)       => `(Com.cat ⦃$x⦄ ⦃$y⦄)
-  | `(⦃if $b {$x} else {$y}⦄) => `(Com.ife ⦃$b⦄ ⦃$x⦄ ⦃$y⦄)
+  | `(⦃if $b {$x} else {$y}⦄) => `(Com.cond ⦃$b⦄ ⦃$x⦄ ⦃$y⦄)
   | `(⦃while $b {$x}⦄) => `(Com.wle ⦃$b⦄ ⦃$x⦄)
 
-#check ⦃z ≔ 4; if 3 ≤ 2 {y ≔ 4 + 2} else {skip}⦄
+#check ⦃z = 4; if 3 <= 2 {y = 4 + 2} else {skip}⦄
 #check ⦃while tt {skip}⦄
 #check ⦃skip⦄
-#check ⦃x ≔ 5⦄
-#check ⦃x ≔ 5; y ≔ 6⦄
-#check ⦃if x = 5 {y ≔ 6} else {z ≔ 7}⦄
-#check ⦃x ≔ 0; while ¬(x = 5) {skip; skip; x ≔ x + 1}⦄
+#check ⦃x = 5⦄
+#check ⦃x = 5; y = 6⦄
+#check ⦃if x == 5 {y = 6} else {z = 7}⦄
+#check ⦃x = 0; while !(x == 5) {skip; skip; x = x + 1}⦄
