Imp/Equivalence.lean
@@ -7,17 +7,17 @@ theorem Com.Nat_imp_Star {cs: Com × State} (h: cs ⟹ t): cs ⇒* (skip, t) := 
   | skip₁ => exact Relation.ReflTransGen.refl
   | ass₁ => exact Relation.ReflTransGen.single Step.ass₁
   | cat₁ _ _ _ ihc ihd => exact Star.cat ihc ihd
-  | ife₁ hb _ ih =>
-    exact Relation.ReflTransGen.head Step.ife₁ (hb ▸ ih)
-  | ife₂ hb _ ih =>
-    exact Relation.ReflTransGen.head Step.ife₁ (hb ▸ ih)
+  | cond₁ hb _ ih =>
+    exact Relation.ReflTransGen.head Step.cond₁ (hb ▸ ih)
+  | cond₂ hb _ ih =>
+    exact Relation.ReflTransGen.head Step.cond₁ (hb ▸ ih)
   | wle₁ _ hb _ _ ihc ihw =>
     apply Relation.ReflTransGen.head Step.wle₁
-    exact Relation.ReflTransGen.head Step.ife₁ (hb ▸ Star.cat ihc ihw)
+    exact Relation.ReflTransGen.head Step.cond₁ (hb ▸ Star.cat ihc ihw)
   | wle₂ hb =>
     apply Relation.ReflTransGen.head Step.wle₁
     apply Relation.ReflTransGen.head _ Relation.ReflTransGen.refl
-    exact (Step.ite_false hb).mpr rfl
+    exact (Step.cond_false hb).mpr rfl
 
 lemma Com.Step_imp_Nat (h₁: cs₀ ⇒ cs₁) (h₂: cs₁ ⟹ s₂): cs₀ ⟹ s₂ := by
   induction h₁ generalizing s₂ with
@@ -26,7 +26,7 @@ lemma Com.Step_imp_Nat (h₁: cs₀ ⇒ cs₁) (h₂: cs₁ ⟹ s₂): cs₀ ⟹
   | cat₂ _ ih =>
     cases h₂ with
     | cat₁ _ hc hd => exact Nat.cat₁ _ (ih hc) hd
-  | ife₁ => exact Nat.ife_ext''.mpr h₂
+  | cond₁ => exact Nat.cond_ext''.mpr h₂
   | wle₁ => rw [Nat.wle_unfold]; exact h₂
 
 theorem Com.Star_imp_Nat (h: cs ⇒* (skip, t)): cs ⟹ t := by
@@ -44,10 +44,10 @@ theorem Com.denot.of_Nat {cs: Com × State} (h : cs ⟹ t):
   | cat₁ t _ _ ih₁ ih₂ =>
     simp at *
     exists t
-  | ife₁ hb _ ih =>
+  | cond₁ hb _ ih =>
     simp at *
     simp [denot, Or.inl, SRel.restrict, hb, ih]
-  | ife₂ hb _ ih =>
+  | cond₂ hb _ ih =>
     simp at *
     simp [denot, Or.inr, SRel.restrict, hb, ih]
   | wle₁ t hb _ _ ih₁ ih₂ =>
@@ -72,19 +72,19 @@ theorem Com.Nat.of_denot (h: (s, t) ∈ ⟦c⟧): (c, s) ⟹ t := by
     intro h
     cases h with | intro w h =>
       exact cat₁ w (ih₁ h.left) (ih₂ h.right)
-  | ife _ _ _ ih₁ ih₂ =>
+  | cond _ _ _ ih₁ ih₂ =>
     intro h
     cases h with
     | inl h =>
       simp at *
       cases h with | intro h hb =>
-        exact ife₁ hb (ih₁ h)
+        exact cond₁ hb (ih₁ h)
     | inr h =>
       simp at *
       cases h with | intro h hb =>
-        exact ife₂ hb (ih₂ h)
+        exact cond₂ hb (ih₂ h)
   | wle b c ih =>
-    suffices ⟦wle b c⟧ ≤ {st | (wle b c, st.1) ⟹ st.2} by apply this
+    suffices ⟦wle b c⟧ ≤ {s | (wle b c, s.1) ⟹ s.2} by apply this
     apply OrderHom.lfp_le
     intro ss h
     cases ss with | mk =>
