Imp/Natural.lean
@@ -5,19 +5,19 @@ inductive Com.Nat: Com × State → State → Prop
     Nat (skip, s) s
 
   | ass₁:
-    Nat (x ≔ a, s) (s⟦x↦a↓s⟧)
+    Nat (ass x a, s) (s⟦x↦a↓s⟧)
 
   | cat₁ t
     (hc: Nat (c, s) t) (hd: Nat (d, t) u):
     Nat (c;;d, s) u
 
-  | ife₁ {b: Bexp}
+  | cond₁ {b: Bexp}
     (hb: b↓s = true) (hc: Nat (c, s) t):
-    Nat (ife b c d, s) t
+    Nat (cond b c d, s) t
 
-  | ife₂ {b: Bexp}
+  | cond₂ {b: Bexp}
     (hb: b↓s = false) (hd: Nat (d, s) t):
-    Nat (ife b c d, s) t
+    Nat (cond b c d, s) t
 
   | wle₁ {b: Bexp} u
     (hb: b↓s = true) (hc: Nat (c, s) u) (hw: Nat (wle b c, u) t):
@@ -29,11 +29,11 @@ inductive Com.Nat: Com × State → State → Prop
 
 infix:110 " ⟹ " => Com.Nat
 
-theorem Com.Nat.demo₁: (⦃x ≔ 5⦄, ⟦⟧) ⟹ ⟦"x"↦5⟧ := ass₁
+theorem Com.Nat.demo₁: (⦃x = 5⦄, ⟦⟧) ⟹ ⟦"x"↦5⟧ := ass₁
 
 theorem Com.Nat.demo₂:
-  (⦃x ≔ 2; if x ≤ 1 {y ≔ 3} else {z ≔ 4}⦄, ⟦⟧) ⟹
-  (⟦"x"↦2⟧⟦"z"↦4⟧) := cat₁ _ ass₁ (ife₂ rfl ass₁)
+  (⦃x = 2; if x <= 1 {y = 3} else {z = 4}⦄, ⟦⟧) ⟹
+  (⟦"x"↦2⟧⟦"z"↦4⟧) := cat₁ _ ass₁ (cond₂ rfl ass₁)
 
 theorem Com.Nat.skip_same: (skip, s) ⟹ s₁ ↔ s = s₁ := ⟨(by cases .; rfl), (· ▸ skip₁)⟩
 
@@ -59,32 +59,32 @@ theorem Com.Nat.skipr: (c;;skip) ≈ c := by
     exact skip_same.mp hd ▸ hc
   . exact (cat₁ _ · skip₁)
 
-theorem Com.Nat.ife_tt (h: b ≈ Bexp.tt): ife b c d ≈ c := by
+theorem Com.Nat.cond_tt (h: b ≈ Bexp.tt): cond b c d ≈ c := by
   intro _ _; constructor <;> intro h₁
   . cases h₁ with
-    | ife₁ => assumption
-    | ife₂ hb => rw [h] at hb; contradiction
-  . apply Nat.ife₁ _ h₁
+    | cond₁ => assumption
+    | cond₂ hb => rw [h] at hb; contradiction
+  . apply Nat.cond₁ _ h₁
     . apply h
 
-theorem Com.Nat.ife_ff (h: b ≈ Bexp.ff): ife b c d ≈ d := by
+theorem Com.Nat.cond_ff (h: b ≈ Bexp.ff): cond b c d ≈ d := by
   intro _ _; constructor <;> intro h₁
   . cases h₁ with
-    | ife₂ => assumption
-    | ife₁ hb => rw [h] at hb; contradiction
-  . apply Nat.ife₂ _ h₁
+    | cond₂ => assumption
+    | cond₁ hb => rw [h] at hb; contradiction
+  . apply Nat.cond₂ _ h₁
     . apply h
 
 theorem Com.Nat.wle_unfold:
-  wle b c ≈ ife b (c;;wle b c) skip := by
+  wle b c ≈ cond b (c;;wle b c) skip := by
   intro s t
   constructor <;> intro h
   . cases hb: b↓s
-    . apply ife₂ hb
+    . apply cond₂ hb
       cases h
       . rw [hb] at *; contradiction
       . constructor
-    . apply ife₁ hb
+    . apply cond₁ hb
       cases h
       . constructor <;> assumption
       . rw [hb] at *; contradiction
@@ -96,7 +96,7 @@ theorem Com.Nat.wle_unfold:
       . rename_i hc; cases hc; constructor <;> assumption
       . rw [hb] at *; contradiction
 
-theorem Com.Nat.ife_ext: (ife b c d, s) ⟹ t ↔ cond (b↓s) ((c, s) ⟹ t) ((d, s) ⟹ t) := by
+theorem Com.Nat.cond_ext: (cond b c d, s) ⟹ t ↔ bif b↓s then (c, s) ⟹ t else (d, s) ⟹ t := by
   constructor <;> intro h <;> cases hb: b↓s <;> simp at *
   . cases h
     simp [hb] at *
@@ -105,15 +105,15 @@ theorem Com.Nat.ife_ext: (ife b c d, s) ⟹ t ↔ cond (b↓s) ((c, s) ⟹ t) ((
     assumption
     simp [hb] at *
   . rw [hb] at h
-    exact ife₂ hb h
+    exact cond₂ hb h
   . rw [hb] at h
-    exact ife₁ hb h
+    exact cond₁ hb h
 
-theorem Com.Nat.ife_ext': (ife b c d, s) ⟹ t ↔ (cond (b↓s) c d, s) ⟹ t := by
-  rw [ife_ext]; cases b↓s <;> simp
+theorem Com.Nat.cond_ext': (cond b c d, s) ⟹ t ↔ (bif b↓s then c else d, s) ⟹ t := by
+  rw [cond_ext]; cases b↓s <;> simp
 
-theorem Com.Nat.ife_ext'': (ife b c d, s) ⟹ t ↔ (cond (b↓s) (c, s) (d, s)) ⟹ t := by
-  rw [ife_ext]; cases b↓s <;> simp
+theorem Com.Nat.cond_ext'': (cond b c d, s) ⟹ t ↔ (bif b↓s then (c, s) else (d, s)) ⟹ t := by
+  rw [cond_ext]; cases b↓s <;> simp
 
 theorem Com.Nat.wle_iff:
   (wle b c, s) ⟹ u ↔
@@ -162,13 +162,13 @@ theorem Com.Nat.determ {cs: Com × State} (h₁: cs ⟹ t) (h₂: cs ⟹ u): t =
   | cat₁ _ _ _ ih₁ ih₂ => cases h₂ with
     | cat₁ _ hc hd => exact ih₂ (ih₁ hc ▸ hd)
 
-  | ife₁ hb _ ih => cases h₂ with
-    | ife₁ _ hd => exact ih hd
-    | ife₂ hb₁ hd => simp [hb] at hb₁
+  | cond₁ hb _ ih => cases h₂ with
+    | cond₁ _ hd => exact ih hd
+    | cond₂ hb₁ hd => simp [hb] at hb₁
 
-  | ife₂ hb _ ih => cases h₂ with
-    | ife₁ hb₁ hd => simp [hb] at hb₁
-    | ife₂ _ hd   => exact ih hd
+  | cond₂ hb _ ih => cases h₂ with
+    | cond₁ hb₁ hd => simp [hb] at hb₁
+    | cond₂ _ hd   => exact ih hd
 
   | wle₁ _ hb _ _ ih₁ ih₂ => cases h₂ with
     | wle₁ _ _ hc hw => exact ih₂ (ih₁ hc ▸ hw)
